theories/utp_circus.thy
@@ -4,7 +4,7 @@
 (* Authors: Simon Foster and Frank Zeyda (University of York, UK)             *)
 (* Emails: simon.foster@york.ac.uk frank.zeyda@york.ac.uk                     *)
 (******************************************************************************)
-(* LAST REVIEWED: 23 June 2017 *)
+(* LAST REVIEWED: 28 June 2017 *)
 
 section {* Theory of {\Circus} *}
 
@@ -39,34 +39,6 @@ definition Process ::
    (unit, '\<epsilon>) action" where
 "Process P = hide_state (\<exists> {$st,$st\<acute>} \<bullet> P)"
 
-lemma Process_eq_simp:
-"(Process P = Process Q) \<longleftrightarrow>
-  ((\<exists> {$st,$st\<acute>} \<bullet> P) = (\<exists> {$st,$st\<acute>} \<bullet> Q))"
-apply (unfold Process_def)
-apply (unfold hide_state_def)
-apply (rel_simp)
-done
-
-lemma Process_ref_simp:
-"(Process P \<sqsubseteq> Process Q) \<longleftrightarrow>
-  ((\<exists> {$st,$st\<acute>} \<bullet> P) \<sqsubseteq> (\<exists> {$st,$st\<acute>} \<bullet> Q))"
-apply (unfold Process_def)
-apply (unfold hide_state_def)
-apply (rel_simp)
-done
-
-lemma Process_eqI:
-"((\<exists> {$st,$st\<acute>} \<bullet> P) = (\<exists> {$st,$st\<acute>} \<bullet> Q)) \<Longrightarrow> (Process P = Process Q)"
-apply (unfold Process_eq_simp)
-apply (assumption)
-done
-
-lemma Process_refI:
-"((\<exists> {$st,$st\<acute>} \<bullet> P) \<sqsubseteq> (\<exists> {$st,$st\<acute>} \<bullet> Q)) \<Longrightarrow> (Process P \<sqsubseteq> Process Q)"
-apply (unfold Process_ref_simp)
-apply (assumption)
-done
-
 text {* The function below makes the state type explicit via an argument. *}
 
 definition ProcessSt ::
@@ -86,7 +58,7 @@ definition RecAction ::
     ('\<sigma>, '\<epsilon>) action \<times> ('\<sigma>, '\<epsilon>) action) \<Rightarrow>
    ('\<sigma>, '\<epsilon>) action" where
 "RecAction act_body =
-  Action (\<mu> X \<bullet> fst (act_body X)) (\<lambda>X. snd (act_body X))"
+  Action (\<mu>\<^sub>C X \<bullet> fst (act_body X)) (\<lambda>X. snd (act_body X))"
 
 lemmas circus_syntax =
   Process_def ProcessSt_def Action_def RecAction_def
@@ -109,7 +81,7 @@ syntax
   "_Action"  :: "[pttrn, logic] \<Rightarrow> action"     ("(2_ =/ _)" 10)
   ""         :: "action \<Rightarrow> actions"            ("_")
   "_Actions" :: "[action, actions] \<Rightarrow> actions" ("_and//_")
-  "_ProcBody" :: "[actions, logic] \<Rightarrow> process" ("((2begin//(_)//\<bullet> (_))//end)")
+  "_ProcBody" :: "[actions, logic] \<Rightarrow> process"          ("((2begin//(_)//\<bullet> (_))//end)")
   "_ProcBodySt" :: "[state, actions, logic] \<Rightarrow> process" ("((2begin//(_)//(_)//\<bullet> (_))//end)")
   "_BasicProc" :: "idt \<Rightarrow> process \<Rightarrow> bool"     ("(process _ \<triangleq>//_)" [0, 10] 10)
   "_BasicDefn" :: "idt \<Rightarrow> logic   \<Rightarrow> bool"     ("(process _ \<triangleq>//_)" [0, 10] 10)
@@ -176,10 +148,6 @@ purge_notation
   ParCSP_NS (infixr "[|_|]" 105) and
   InterleaveCSP (infixr "|||" 105)
 
-purge_syntax
-  "_output_prefix" :: "('a, '\<sigma>) uexpr \<Rightarrow> prefix_elem'" ("!'(_')")
-  "_output_prefix" :: "('a, '\<sigma>) uexpr \<Rightarrow> prefix_elem'" (".'(_')")
-
 consts ParCircus ::
   "('\<sigma>, '\<phi>) action  \<Rightarrow> ('\<phi> event set) \<Rightarrow> ('\<sigma>, '\<phi>) action \<Rightarrow>
    ('\<sigma>, '\<phi>) action" (infixl "[|(_)|]" 60)
@@ -195,261 +163,6 @@ consts HideCircus ::
 consts InterruptCircus ::
   "('\<sigma>, '\<phi>) action  \<Rightarrow> ('\<sigma>, '\<phi>) action \<Rightarrow> ('\<sigma>, '\<phi>) action" (infixl "\<triangle>" 100)
 
-subsection {* Input Prefix (OLD) *}
-
-(*
-definition do\<^sub>I :: "
-  ('a, '\<epsilon>) chan \<Rightarrow>
-  ('a \<Longrightarrow> ('\<sigma>, '\<epsilon>) st_csp) \<Rightarrow>
-  ('a \<Rightarrow> ('\<sigma>, '\<epsilon>) action) \<Rightarrow>
-  ('\<sigma>, '\<epsilon>) action" where
-"do\<^sub>I c x P =
-  (($tr\<acute> =\<^sub>u $tr \<and> {e : \<guillemotleft>\<delta>\<^sub>u(c)\<guillemotright> | P(e) \<bullet> (c\<cdot>\<guillemotleft>e\<guillemotright>)\<^sub>u}\<^sub>u \<inter>\<^sub>u $ref\<acute> =\<^sub>u {}\<^sub>u)
-    \<triangleleft> $wait\<acute> \<triangleright>
-  (($tr\<acute> - $tr) \<in>\<^sub>u {e : \<guillemotleft>\<delta>\<^sub>u(c)\<guillemotright> | P(e) \<bullet> \<langle>(c\<cdot>\<guillemotleft>e\<guillemotright>)\<^sub>u\<rangle>}\<^sub>u \<and> (c\<cdot>$x\<acute>)\<^sub>u =\<^sub>u last\<^sub>u($tr\<acute>)))"
-*)
-
-definition InputCircus ::
-  "('a::{continuum, two}, '\<epsilon>) chan \<Rightarrow>
-    ('a, ('\<sigma>, '\<epsilon>) st_csp) lvar \<Rightarrow>
-    ('a \<Rightarrow> ('\<sigma>, '\<epsilon>) action) \<Rightarrow>
-    (('a \<Longrightarrow> ('\<sigma>, '\<epsilon>) st_csp) \<Rightarrow> ('\<sigma>, '\<epsilon>) action) \<Rightarrow>
-    ('\<sigma>, '\<epsilon>) action" where
-"InputCircus c x P A =
-  (var\<^bsub>RDES\<^esub> x \<bullet> \<^bold>R\<^sub>s(true \<turnstile> (do\<^sub>I c x P) \<and> (\<exists> $x\<acute> \<bullet> II)) ;; A(x))"
-
-text {* A few syntactic adjustments, remove them and adapt @{text "fmi.thy"}. *}
-
-no_notation utp_rel_opsem.trel (infix "\<rightarrow>\<^sub>u" 85)
-
-syntax
-  "_circus_sync" :: "logic \<Rightarrow> logic \<Rightarrow> logic" (infixl "\<rightarrow>\<^sub>u" 80)
-  "_circus_input" :: "logic \<Rightarrow> id \<Rightarrow> logic \<Rightarrow> logic \<Rightarrow> logic"
-    ("_?\<^sub>u'(_ :/ _') \<rightarrow> _" [81, 0, 0, 80] 80)
-  "_circus_output" :: "logic \<Rightarrow> logic \<Rightarrow> logic \<Rightarrow> logic"
-    ("_!\<^sub>u'(_') \<rightarrow> _" [81, 0, 80] 80)
-
-translations
-  "c \<rightarrow>\<^sub>u A" \<rightleftharpoons> "(CONST OutputCSP) c ()\<^sub>u A"
-  "c!\<^sub>u(v) \<rightarrow> A" \<rightleftharpoons> "(CONST OutputCSP) c v A"
-  "c?\<^sub>u(x : P) \<rightarrow> A" \<rightharpoonup> "(CONST InputCircus) c
-    (*(CONST top_var \<dots>*) (CONST MkDVar IDSTR(x)) (\<lambda>x. P) (\<lambda>x. A)"
-  "c?\<^sub>u(x : P) \<rightarrow> A" \<leftharpoondown> "(CONST InputCircus) c x (\<lambda>v. P) (\<lambda>w. A)"
-
-subsection {* Mixed Prefixes *}
-
-text {* In this section, we provide support for mixed prefixes. *}
-
-(*
-syntax
-  "_circus_sync" :: "logic \<Rightarrow> logic \<Rightarrow> logic" ("_ \<rightarrow> _" [81, 80] 80)
-  "_circus_output" :: "logic \<Rightarrow> logic \<Rightarrow> logic \<Rightarrow> logic"
-    ("_!\<^sub>u'(_') \<rightarrow> _" [81, 0, 80] 80)
-  "_circus_input"  :: "logic \<Rightarrow> id \<Rightarrow> logic \<Rightarrow> logic \<Rightarrow> logic"
-    ("_?\<^sub>u'(_ :/ _') \<rightarrow> _" [81, 0, 0, 80] 80)
-*)
-(*
-no_translations
-  "c \<^bold>\<rightarrow> A"      \<leftharpoondown> "(CONST OutputCSP) c ()\<^sub>u A"
-  "c!\<^sub>u(v) \<rightarrow> A" \<leftharpoondown> "(CONST OutputCSP) c v A"
-*)
-
-subsubsection {* Prefix Semantics *}
-
-text {*
-  We first define a new and simplified version of the @{const InputCircus}
-  operator. Simplification is due to its action argument being parametrised
-  by the a (HOL) value rather than a variable lens. This makes a subsequent
-  definition of syntax and translations for mixed prefixes much easier. We
-  note that all different kinds of prefixes will be expressed in terms of
-  input communications with appropriate constraints on variables that are
-  introduced by the prefix construct.
-*}
-
-definition new_do\<^sub>I :: "
-  ('a, '\<epsilon>) chan \<Rightarrow> 'a \<Rightarrow>
-  ('a \<Rightarrow> ('\<sigma>, '\<epsilon>) action) \<Rightarrow>
-  ('\<sigma>, '\<epsilon>) action" where
-"new_do\<^sub>I c x P =
-  (($tr\<acute> =\<^sub>u $tr \<and> {e : \<guillemotleft>\<delta>\<^sub>u(c)\<guillemotright> | P(e) \<bullet> (c\<cdot>\<guillemotleft>e\<guillemotright>)\<^sub>u}\<^sub>u \<inter>\<^sub>u $ref\<acute> =\<^sub>u {}\<^sub>u)
-    \<triangleleft> $wait\<acute> \<triangleright>
-  (($tr\<acute> - $tr) \<in>\<^sub>u {e : \<guillemotleft>\<delta>\<^sub>u(c)\<guillemotright> | P(e) \<bullet> \<langle>(c\<cdot>\<guillemotleft>e\<guillemotright>)\<^sub>u\<rangle>}\<^sub>u \<and> (c\<cdot>\<guillemotleft>x\<guillemotright>)\<^sub>u =\<^sub>u last\<^sub>u($tr\<acute>)))"
-
-definition new_do\<^sub>I' :: "
-  ('a, '\<epsilon>) chan \<Rightarrow> 'a \<Rightarrow>
-  ('a \<Rightarrow> ('\<sigma>, '\<epsilon>) action) \<Rightarrow>
-  ('\<sigma>, '\<epsilon>) action" where
-"new_do\<^sub>I' c x P =
-  (($tr\<acute> =\<^sub>u $tr \<and> (c\<cdot>\<guillemotleft>x\<guillemotright>)\<^sub>u \<notin>\<^sub>u $ref\<acute>) \<triangleleft> $wait\<acute> \<triangleright> (($tr\<acute> - $tr) =\<^sub>u \<langle>(c\<cdot>\<guillemotleft>x\<guillemotright>)\<^sub>u\<rangle>))"
-
-definition NewInputCircus ::
-  "('a, '\<epsilon>) chan \<Rightarrow>
-    ('a \<Rightarrow> ('\<sigma>, '\<epsilon>) action) \<Rightarrow>
-    ('a \<Rightarrow> ('\<sigma>, '\<epsilon>) action) \<Rightarrow>
-    ('\<sigma>, '\<epsilon>) action" where
-"NewInputCircus c P A = (\<^bold>\<exists> x \<bullet> \<^bold>R\<^sub>s(true \<turnstile> (new_do\<^sub>I c x P) \<and> II) ;; A(x))"
-
-definition NewInputCircus' ::
-  "('a, '\<epsilon>) chan \<Rightarrow>
-    ('a \<Rightarrow> ('\<sigma>, '\<epsilon>) action) \<Rightarrow>
-    ('a \<Rightarrow> ('\<sigma>, '\<epsilon>) action) \<Rightarrow>
-    ('\<sigma>, '\<epsilon>) action" where
-"NewInputCircus' c P A = (\<^bold>\<exists> x \<bullet> \<^bold>R\<^sub>s(true \<turnstile> (new_do\<^sub>I' c x P) \<and> II) ;; A(x))"
-
-lemma "NewInputCircus = NewInputCircus'"
-apply (rule ext)+
-apply (unfold NewInputCircus_def NewInputCircus'_def)
-apply (unfold new_do\<^sub>I_def new_do\<^sub>I'_def)
--- {* TODO: Allow simplification theorems to be passed to rel\_simp. *}
-apply (rel_simp)
-apply (safe; clarsimp?)
-apply (blast)
-apply (simp_all add: zero_list_def)    
-apply (blast)
-apply (metis)
-apply (metis)
-apply (blast)
-apply (blast)
-apply (metis)+
-done
-
-(* Need to figure out how to state the law below... ?! *)
-
-lemma
-"vwb_lens x \<Longrightarrow> NewInputCircus c P A = InputCircus c x P B"
-apply (unfold NewInputCircus_def InputCircus_def)
-apply (unfold new_do\<^sub>I_def do\<^sub>I_def chan_type_def)
-apply (rel_simp)
-apply (safe; clarsimp simp add: comp_def)
-oops
-
-subsubsection {* Syntax and Translations *}
-
-text {* We next configure a syntax for mixed prefixes. *}
-
-nonterminal prefix_elem and mixed_prefix
-
-syntax "" :: "prefix_elem \<Rightarrow> mixed_prefix" ("_")
-
-text {* Input Prefix: @{text "\<dots>?(x)"} *}
-
-syntax "_simple_input_prefix" :: "id \<Rightarrow> prefix_elem"  ("?'(_')")
-
-text {* Input Prefix with Constraint: @{text "\<dots>?(x : P)"} *}
-
-syntax "_input_prefix" :: "id \<Rightarrow> ('\<sigma>, '\<epsilon>) action \<Rightarrow> prefix_elem" ("?'(_ :/ _')")
-
-text {* Output Prefix: @{text "\<dots>![v]e"} *}
-
-text {* A variable name must currently be provided for outputs, too. Fix?! *}
-
-syntax "_output_prefix" :: "id \<Rightarrow> ('a, '\<sigma>) uexpr \<Rightarrow> prefix_elem" ("![_]_")
-syntax "_output_prefix" :: "id \<Rightarrow> ('a, '\<sigma>) uexpr \<Rightarrow> prefix_elem" (".[_]_")
-
-syntax (output) "_output_prefix_pp" :: "('a, '\<sigma>) uexpr \<Rightarrow> prefix_elem" ("!_")
-
-text {* Synchronisation Action: @{text "c \<rightarrow>\<^sub>\<C> A"} *}
-
-syntax "_sync_action" ::
-  "('a, '\<epsilon>) chan \<Rightarrow> ('\<sigma>, '\<epsilon>) action \<Rightarrow> ('\<sigma>, '\<epsilon>) action" (infixr "\<rightarrow>\<^sub>\<C>" 80)
-
-text {* Mixed-Prefix Action: @{text "c\<dots>(prefix) \<rightarrow>\<^sub>\<C> A"} *}
-
-syntax "_mixed_prefix" :: "prefix_elem \<Rightarrow> mixed_prefix \<Rightarrow> mixed_prefix" ("__")
-
-syntax "_prefix_action" ::
-  "('a, '\<epsilon>) chan \<Rightarrow> mixed_prefix \<Rightarrow> ('\<sigma>, '\<epsilon>) action \<Rightarrow> ('\<sigma>, '\<epsilon>) action"
-  ("(__ \<rightarrow>\<^sub>\<C>/ _)" [81, 81, 80] 80)
-
-text {* Syntax translations *}
-
-translations
-  "_simple_input_prefix x" \<rightleftharpoons> "_input_prefix x true"
-  "_output_prefix x e" \<rightharpoonup> "_input_prefix x (\<guillemotleft>x\<guillemotright> =\<^sub>u e)"
-  "_output_prefix_pp e" \<leftharpoondown> "_input_prefix v (\<guillemotleft>x\<guillemotright> =\<^sub>u e)" (* Better do in ML! *)
-
-translations
-  "_mixed_prefix (_input_prefix x P) (_input_prefix y Q)" \<rightleftharpoons>
-  "_input_prefix (_pattern x y) (P \<and> Q)"
-
-translations
-  "_sync_action c A" \<rightleftharpoons> "(CONST OutputCSP) c ()\<^sub>u A"
-  "_prefix_action c (_input_prefix x P) A"  \<rightharpoonup>
-  "(CONST NewInputCircus) c (\<lambda>x. P) (\<lambda>x. A)"
-(* "_prefix_action c (_input_prefix x P) A"  \<leftharpoondown>
-  "(CONST NewInputCircus) c (\<lambda>x. P) (\<lambda>v. A)" *)
-
-text {*
-  The ML print translation for @{const NewInputCircus} below is a little more
-  robust than using Isabelle in-built @{command translations} in dealing with
-  unwanted eta-contraction.
-*}
-
-ML {*
-signature CIRCUS_PREFIX =
-sig
-  val mk_pattern: term list -> term
-  val strip_abs_tr': term list -> term -> term list * term
-  val mk_input_prefix: term -> term -> term
-  val mk_prefix_action: term -> term -> term -> term -> term
-  val InputCircus_tr': term list -> term
-end;
-
-structure Circus_Prefix : CIRCUS_PREFIX =
-struct
-  fun mk_pattern [] = Const (@{syntax_const "_unit"}, dummyT)
-  | mk_pattern [x] = x
-  | mk_pattern (h :: t) =
-    Const (@{syntax_const "_pattern"}, dummyT) $ h $ (mk_pattern t);
-
-  fun strip_abs_tr' vs (Abs abs) =
-    let val (v, body) = Syntax_Trans.atomic_abs_tr' abs in
-      strip_abs_tr' (vs @ [v]) body
-    end
-  | strip_abs_tr' vs
-      (Const (@{const_syntax case_prod}, _) $ (Abs abs)) =
-    let val (v, body) = Syntax_Trans.atomic_abs_tr' abs in
-      strip_abs_tr' (vs @ [v]) body
-    end
-  | strip_abs_tr' vs term = (vs, term);
-
-  fun mk_input_prefix x P =
-    Const (@{syntax_const "_input_prefix"}, dummyT) $ x $ P;
-
-  fun mk_prefix_action c x P A =
-    Const (@{syntax_const "_prefix_action"}, dummyT) $ c $
-      (mk_input_prefix x P) $ A;
-
-  fun InputCircus_tr' [c, P, A] = let
-    val (vs, P') = strip_abs_tr' [] P;
-    val (vs', A') = strip_abs_tr' [] A in
-      if (vs = vs') then
-        (mk_prefix_action c (mk_pattern vs) P' A')
-      else raise Match
-    end
-  | InputCircus_tr' _ = raise Match;
-end;
-*}
-
-print_translation {*
-  [(@{const_syntax NewInputCircus}, K Circus_Prefix.InputCircus_tr')]
-*}
-
-text {* Testing *}
-
-text {* All of the below seem to work! *}
-
-term "c?(x : true) \<rightarrow>\<^sub>\<C> A x"
-term "c?(x : true)?(y : true) \<rightarrow>\<^sub>\<C> A x y"
-term "c?(x : true)?(y : true)?(z : true) \<rightarrow>\<^sub>\<C> A x y z"
-term "c?(x : \<guillemotleft>x\<guillemotright> <\<^sub>u \<guillemotleft>10::nat\<guillemotright>) \<rightarrow>\<^sub>\<C> A x"
-term "c?(x)?(y : true) \<rightarrow>\<^sub>\<C> A x y"
-term "c?(x : true)![st]\<guillemotleft>1::nat\<guillemotright> \<rightarrow>\<^sub>\<C> A x"
-term "c![st]\<guillemotleft>1::nat\<guillemotright>?(x : true) \<rightarrow>\<^sub>\<C> A x"
-term "c![st]\<guillemotleft>1::nat\<guillemotright> \<rightarrow>\<^sub>\<C> A"
-term "c![x]\<guillemotleft>1::nat\<guillemotright>![y]\<guillemotleft>2::nat\<guillemotright> \<rightarrow>\<^sub>\<C> A"
-term "c \<rightarrow>\<^sub>\<C> A"
-
 subsection {* Circus Conditional *}
 
 syntax "_if_then_else" ::
@@ -461,7 +174,7 @@ translations "if\<^sub>\<C> b then\<^sub>\<C> P else\<^sub>\<C> Q" \<rightleftha
 subsection {* Iterated Constructs *}
 
 text {* In this section, we define various iterated constructs. *}
-  
+
 subsubsection {* Iterated Interleaving *}
 
 primrec interleave_iter ::
@@ -486,7 +199,7 @@ theorem
  P = Process (Main (Act1, Act2 ;; Act1))"
 apply (unfold circus_syntax)
 apply (unfold Let_def) -- {* \todo{How to apply the copy rule selectively?!} *}
-apply (clarsimp)
+apply (simp add: o_def)
 done
 
 theorem
@@ -494,7 +207,7 @@ theorem
  P = ProcessSt TYPE(vstore) (Main (Act1, Act2 ;; Act1))"
 apply (unfold circus_syntax)
 apply (unfold Let_def) -- {* \todo{How to apply the copy rule selectively?!} *}
-apply (clarsimp)
+apply (simp add: o_def)
 done
 
 theorem
@@ -502,6 +215,45 @@ theorem
  P = (\<lambda>x. ProcessSt TYPE('\<sigma>) (Main (Act1 x, Act2 ;; Act1 x)))"
 apply (unfold circus_syntax)
 apply (unfold Let_def) -- {* \todo{How to apply the copy rule selectively?!} *}
-apply (clarsimp)
+apply (simp add: o_def)
+done
+
+subsection {* Supplementary Laws *}
+
+lemma all_true [simp]:
+"(\<forall> x \<bullet> true) = true"
+apply(pred_auto)
+done
+
+text \<open>Simplification laws for processes with the same state type.\<close>
+
+lemma Process_eq_simp:
+"(Process P = Process Q) \<longleftrightarrow>
+  ((\<exists> {$st, $st\<acute>} \<bullet> P) = (\<exists> {$st, $st\<acute>} \<bullet> Q))"
+apply (unfold Process_def)
+apply (unfold hide_state_def)
+apply (rel_simp)
+done
+
+lemma Process_ref_simp:
+"(Process P \<sqsubseteq> Process Q) \<longleftrightarrow>
+  ((\<exists> {$st, $st\<acute>} \<bullet> P) \<sqsubseteq> (\<exists> {$st, $st\<acute>} \<bullet> Q))"
+apply (unfold Process_def)
+apply (rel_simp)
+done
+
+lemma preR_ex_st_vars [rdes]:
+"pre\<^sub>R(\<exists> {$st, $st\<acute>} \<bullet> P) = (\<forall> {$st, $st\<acute>} \<bullet> pre\<^sub>R P)"
+apply (rel_auto)
+done
+
+lemma periR_ex_st_vars [rdes]:
+"peri\<^sub>R(\<exists> {$st, $st\<acute>} \<bullet> P) = (\<exists> {$st, $st\<acute>} \<bullet> peri\<^sub>R P)"
+apply (rel_auto)
+done
+
+lemma postR_ex_st_vars [rdes]:
+"post\<^sub>R(\<exists> {$st, $st\<acute>} \<bullet> P) = (\<exists> {$st, $st\<acute>} \<bullet> post\<^sub>R P)"
+apply (rel_auto)
 done
 end
